Translating to 'pre-fancy' form now works on Montgomery

src/Experiments/SimplyTypedArithmetic.v
@@ -1797,6 +1797,18 @@ Module BaseConversion.
       push_eval.
     Qed.
 
+    (* bind the input, but *not* the carrying operations *)
+    Derive from_associational_inlined
+           SuchThat (forall n idxs p,
+                        from_associational_inlined n idxs p = from_associational n idxs p)
+           As from_associational_inlined_correct.
+    Proof.
+      intros.
+      cbv beta iota delta [from_associational Associational.carry Associational.carryterm].
+      unfold Let_In at 2 3.
+      subst from_associational_inlined; reflexivity.
+    Qed.
+
     (* carry chain that aligns terms in the intermediate weight with the final weight *)
     Definition aligned_carries (log_dw_sw nout : nat)
       := (map (fun i => ((log_dw_sw * (i + 1)) - 1))%nat (seq 0 nout)).
@@ -1857,6 +1869,23 @@ Module BaseConversion.
       autorewrite with zsimplify.
       rewrite Z.pow_mul_r, Z.pow_2_r by omega.
       Z.rewrite_mod_small. reflexivity.
+    Qed.
+
+    Derive widemul_inlined
+           SuchThat (forall a b,
+                        0 <= a * b < 2^log2base * 2^log2base ->
+                        widemul_inlined a b = [(a * b) mod 2^log2base; (a * b) / 2^log2base])
+           As widemul_inlined_correct.
+    Proof.
+      intros.
+      rewrite <-widemul_correct by auto.
+      cbv beta iota delta [widemul mul_converted to_associational convert_bases
+                                   chained_carries_no_reduce carry
+                                   Associational.carry Associational.carryterm
+                                   Positional.from_associational].
+      cbv beta iota delta [Let_In].
+      rewrite <-from_associational_inlined_correct.
+      subst widemul_inlined; reflexivity.
     Qed.
   End widemul.
 End BaseConversion.
@@ -8493,7 +8522,6 @@ barrett_red256 = fun var : type -> Type => λ x : var (type.type_primitive type.
                  ADDM (x43, 0, 115792089210356248762697446949407573530086143415290314195533631308867097853951)
      : Expr (type.uncurry (type.type_primitive type.Z -> type.type_primitive type.Z -> type.type_primitive type.Z))
   *)
-
 End Barrett256.
 
 Module SaturatedSolinas.
@@ -8901,30 +8929,39 @@ Module Straightline.
 
       Let uexpr t := @Uncurried.expr.expr ident.ident var t.
 
-      Inductive expr : type.type -> Type :=
-      | Scalar {t} : scalar t -> expr t
-      | LetInAppIdentZ {s d} : zrange -> ident.ident s (type.Z) -> scalar s -> (var (type.Z) -> expr d) -> expr d
-      | LetInAppIdentZZ {s d} : zrange * zrange -> ident.ident s (type.Z*type.Z) -> scalar s -> (var (type.Z*type.Z) -> expr d) -> expr d
-      with scalar : type.type -> Type :=
-           | Var t : var t -> scalar t
-           | TT : scalar (type.type_primitive type.unit)
-           | Pair {a b} : scalar a -> scalar b -> scalar (a * b)
-           | Cast : zrange -> scalar type.Z -> scalar type.Z
-           | Cast2 : zrange * zrange -> scalar (type.Z*type.Z) -> scalar (type.Z*type.Z)
-           | Fst {a b} : scalar (a * b) -> scalar a
-           | Snd {a b} : scalar (a * b) -> scalar b
-           | Primitive {t} : type.interp (type.type_primitive t) -> scalar t
-      .
+      Section with_ident.
+        Context {ident : type.type -> type.type -> Type}.
+        Inductive expr : type.type -> Type :=
+        | Scalar {t} : scalar t -> expr t
+        | LetInAppIdentZ {s d} : zrange -> ident s (type.Z) -> scalar s -> (var (type.Z) -> expr d) -> expr d
+        | LetInAppIdentZZ {s d} : zrange * zrange -> ident s (type.Z*type.Z) -> scalar s -> (var (type.Z*type.Z) -> expr d) -> expr d
+        with scalar : type.type -> Type :=
+             | Var t : var t -> scalar t
+             | TT : scalar (type.type_primitive type.unit)
+             | Pair {a b} : scalar a -> scalar b -> scalar (a * b)
+             | Cast : zrange -> scalar type.Z -> scalar type.Z
+             | Cast2 : zrange * zrange -> scalar (type.Z*type.Z) -> scalar (type.Z*type.Z)
+             | Fst {a b} : scalar (a * b) -> scalar a
+             | Snd {a b} : scalar (a * b) -> scalar b
+             | Shiftr : Z -> scalar type.Z -> scalar type.Z
+             | Shiftl : Z -> scalar type.Z -> scalar type.Z
+             | Land : Z -> scalar type.Z -> scalar type.Z
+             | Primitive {t} : type.interp (type.type_primitive t) -> scalar t
+        .
+      End with_ident.
 
-      Fixpoint dummy t : expr t := Scalar (Var t (dummy_var t)).
+      Fixpoint dummy t : @expr ident.ident t := Scalar (Var t (dummy_var t)).
 
       Definition scalar_of_uncurried_ident {s d} (idc : ident.ident s d)
         : scalar s -> option (scalar d) :=
-        match idc in ident.ident s d return scalar s -> option (scalar d) with
+        match idc in ident.ident s d return scalar (ident:=ident.ident) s -> option (scalar d) with
         | ident.Z.cast r => fun args => Some (Cast r args)
         | ident.Z.cast2 r => fun args => Some (Cast2 r args)
-        | @ident.fst A B => fun args => Some (@Fst A B args)
-        | @ident.snd A B => fun args => Some (@Snd A B args)
+        | @ident.fst A B => fun args => Some (Fst args)
+        | @ident.snd A B => fun args => Some (Snd args)
+        | ident.Z.shiftr n => fun args => Some (Shiftr n args)
+        | ident.Z.shiftl n => fun args => Some (Shiftl n args)
+        | ident.Z.land n => fun args => Some (Land n args)
         | @ident.primitive p x => fun _ => Some (Primitive x)
         | _ => fun _ => None
         end.
@@ -9000,9 +9037,9 @@ Module Straightline.
         : range_type d -> ident.ident s d -> scalar s -> (var d -> expr t) -> expr t :=
         match d as d0 return range_type d0 -> ident.ident s d0 -> scalar s -> (var d0 -> expr t) -> expr t with
         | type.type_primitive type.Z =>
-          fun r idc x k => @LetInAppIdentZ s t r idc x k
+          fun r idc x k => @LetInAppIdentZ ident.ident s t r idc x k
         | type.prod type.Z type.Z =>
-          fun r idc x k => @LetInAppIdentZZ s t r idc x k
+          fun r idc x k => @LetInAppIdentZZ ident.ident s t r idc x k
         | _ => fun _ _ _ _ => default
         end.
 
@@ -9107,89 +9144,151 @@ Module StraightlineTest.
   Eval vm_compute in (Straightline.of_Expr test_mul).
 End StraightlineTest.
 
-(*
-Module InlineOperations.
+(* Convert straightline code to code that uses only a certain set of identifiers *)
+Module PreFancy.
   Section with_var.
-    Context {var : type.type -> Type} (op_match : forall t, @expr.expr ident.ident var t -> bool).
+    Import Straightline.expr.
+    Context {var : type -> Type} (dummy_var : forall t, var t) (log2wordsize : Z)
+            (constant_to_scalar : forall ident, Z -> option (@scalar var ident type.Z)).
+    Local Notation Z := (type.type_primitive type.Z).
+    Let wordsize := 2 ^ log2wordsize.
+    Let half_bits := log2wordsize / 2.
+    Let half_wordsize := 2 ^ half_bits.
 
-    Fixpoint inline_op {t} (e : @expr.expr ident.ident var t) : @expr.expr ident.ident var t
-      :=
-        match e in expr.expr t return @expr.expr ident.ident var t with
-        | Var t _ as e => e
-        | TT as e
-          => e
-        | Pair A B a b
-          => Pair (@inline_op A a) (@inline_op B b)
-        | App s d f x => App (@inline_op _ f) (@inline_op _ x)
-        | Abs s d f => Abs (fun v => @inline_op _ (f v))
-        | AppIdent s d idc args
-          => inline_op_ident idc (@inline_op s args)
-        end.
+    Inductive ident : type -> type -> Type :=
+    | add : ident (Z * Z) (Z * Z)
+    | addc : ident (Z * Z * Z) (Z * Z)
+    | mulll : ident (Z * Z) Z
+    | mullh : ident (Z * Z) Z
+    | mulhl : ident (Z * Z) Z
+    | mulhh : ident (Z * Z) Z
+    | sub : ident (Z * Z) (Z * Z)
+    | shiftr : BinInt.Z -> ident Z Z
+    | shiftl : BinInt.Z -> ident Z Z
+    | sel : ident (Z * Z * Z) Z
+    | addm : ident (Z * Z * Z) Z
+    .
+    Let dummy t : @expr var ident t := Scalar (Var _ (dummy_var t)).
 
-    (*
-       AppIdent ident.Let_In (Pair (AppIdent (ident.shiftr n) x) (Abs (fun y : var _ => F (Var _ y))))
-
-       =>
-
-       F (AppIdent (ident.shiftr n) x)
-     *)
-
-
-    Definition replace_num {t} (old : var type.Z) (new : @expr.expr ident.ident var type.Z) (e : @expr.expr ident.ident var t)
-      : @expr.expr ident.ident var t
-      := match e with
-         | Var _ v =>
-         | TT => TT
-                   |
-
-
-    Definition inline_if_match {tx tC} (args : @expr.expr ident.ident var (tx * (tx -> tC)))
-      : @expr.expr ident.ident var tC :=
-      let default _ := AppIdent (@ident.Let_In tx tC) args in
-      match invert_Pair args with
-      | Some (e, Abs s d k) =>
-        if op_match tx e then App k e else default tt
-      | None => default tt
+    Definition invert_lower' {t} (e : @scalar var ident t) :
+      option (@scalar var ident Z) :=
+      match e in scalar t return option (@scalar var ident Z) with
+      | Cast r (Land n x) =>
+        if (lower r =? 0) && (upper r =? (half_wordsize - 1)) && (n =? 2^half_bits-1)
+        then Some x
+        else None
+      | _ => None
       end.
 
-    Definition inline_op_ident {s d} (idc : ident.ident s d)
-      : expr.expr s -> expr.expr d
-      :=
-        match idc in ident.ident s d return @expr.expr ident.ident var s -> expr.expr d with
-        | ident.Let_In tx tC => fun args : @expr.expr ident.ident var (tx * (tx -> tC)) =>
-                                  @inline_if_match tx tC args
-        | _ as i => fun args => AppIdent i args
-        end.
+    Definition invert_upper' {t} (e : @scalar var ident t) :
+      option (@scalar var ident Z) :=
+      match e in scalar t return option (@scalar var ident Z) with
+      | Cast r (Shiftr n x) =>
+        if (lower r =? 0) && (upper r =? (half_wordsize - 1)) && (n =? half_bits)
+        then Some x
+        else None
+      | _ => None
+      end.
 
-    Fixpoint inline_op {t} (e : @expr.expr ident.ident var t) : @expr.expr ident.ident var t
-      :=
-        match e in expr.expr t return @expr.expr ident.ident var t with
-        | Var t _ as e => e
-        | TT as e
-          => e
-        | Pair A B a b
-          => Pair (@inline_op A a) (@inline_op B b)
-        | App s d f x => App (@inline_op _ f) (@inline_op _ x)
-        | Abs s d f => Abs (fun v => @inline_op _ (f v))
-        | AppIdent s d idc args
-          => inline_op_ident idc (@inline_op s args)
-        end.
+    Definition invert_lower {t} (e : @scalar var ident t) :
+      option (@scalar var ident Z) :=
+      match e in scalar t return option (@scalar var ident Z) with
+      | Primitive type.Z x =>
+        match constant_to_scalar ident x with
+        | Some y => invert_lower' y
+        | None => None
+        end
+      | _ => invert_lower' e
+      end.
+
+    Definition invert_upper {t} (e : @scalar var ident t) :
+      option (@scalar var ident Z) :=
+      match e in scalar t return option (@scalar var ident Z) with
+      | Primitive type.Z x =>
+        match constant_to_scalar ident x with
+        | Some y => invert_upper' y
+        | None => None
+        end
+      | _ => invert_upper' e
+      end.
+
+
+    Definition of_straightline_ident {s d} (idc : ident.ident s d)
+      : forall t, range_type d -> @scalar var ident s -> (var d -> @expr var ident t) -> @expr var ident t :=
+      match idc in ident.ident s d return forall t, range_type d -> scalar s -> (var d -> @expr var ident t) -> @expr var ident t with
+      | ident.Z.add_get_carry_concrete w =>
+        fun t r x f =>
+          if w =? wordsize
+          then LetInAppIdentZZ r add x f
+          else dummy _
+      | ident.Z.add_with_get_carry_concrete w =>
+        fun t r x f =>
+          if w =? wordsize
+          then LetInAppIdentZZ r addc x f
+          else dummy _
+      | ident.Z.sub_get_borrow_concrete w =>
+        fun t r x f =>
+          if w =? wordsize
+          then LetInAppIdentZZ r sub x f
+          else dummy _
+      | ident.Z.shiftr n => fun _ r => LetInAppIdentZ r (shiftr n)
+      | ident.Z.shiftl n => fun _ r => LetInAppIdentZ r (shiftl n)
+      | ident.Z.zselect => fun _ r => LetInAppIdentZ r sel
+      | ident.Z.add_modulo => fun _ r => LetInAppIdentZ r addm
+      | ident.Z.mul =>
+        fun t r x f =>
+          match x return expr t with
+          | Pair _ _ x0 x1 =>
+            match invert_lower x0, invert_lower x1 with
+            | Some y0, Some y1 => LetInAppIdentZ r mulll (Pair y0 y1) f
+            | Some y0, None =>
+              match invert_upper x1 with
+              | Some y1 => LetInAppIdentZ r mullh (Pair y0 y1) f
+              | None => dummy _
+              end
+            | None, Some y1 =>
+              match invert_upper x0 with
+              | Some y0 => LetInAppIdentZ r mulhl (Pair y0 y1) f
+              | None => dummy _
+              end
+            | None, None =>
+              match invert_upper x0, invert_upper x1 with
+              | Some y0, Some y1 => LetInAppIdentZ r mulhh (Pair y0 y1) f
+              | _,_ => dummy _
+              end
+            end
+          | _ => dummy _
+          end
+      | _ => fun t _ _ _ => dummy t
+      end.
+
+    Fixpoint of_straightline_scalar {t} (s : @scalar var ident.ident t)
+      : @scalar var ident t :=
+      match s with
+      | Var _ v => Var _ v
+      | TT => TT
+      | Pair _ _ x y => Pair (of_straightline_scalar x) (of_straightline_scalar y)
+      | Cast r x => Cast r (of_straightline_scalar x)
+      | Cast2 r x => Cast2 r (of_straightline_scalar x)
+      | Fst _ _ x => Fst (of_straightline_scalar x)
+      | Snd _ _ x => Snd (of_straightline_scalar x)
+      | Shiftr n x => Shiftr n (of_straightline_scalar x)
+      | Shiftl n x => Shiftl n (of_straightline_scalar x)
+      | Land n x => Land n (of_straightline_scalar x)
+      | Primitive _ x => Primitive x
+      end.
+
+    Fixpoint of_straightline {t} (e : @expr var ident.ident t)
+      : @expr var ident t :=
+      match e with
+      | Scalar _ s => Scalar (of_straightline_scalar s)
+      | LetInAppIdentZ _ t r idc x f =>
+        of_straightline_ident idc t r (of_straightline_scalar x) (fun y => of_straightline (f y))
+      | LetInAppIdentZZ _ t r idc x f =>
+        of_straightline_ident idc t r (of_straightline_scalar x) (fun y => of_straightline (f y))
+      end.
   End with_var.
-
-  Fixpoint shift_land_matcher {var} t (e : @expr.expr ident.ident var t) : bool :=
-    match e with
-    | AppIdent _ _ (ident.Z_cast _) args => shift_land_matcher _ args
-    | AppIdent _ _ (ident.Z_cast2 _) args => shift_land_matcher _ args
-    | AppIdent _ _ (ident.Z_land _) args => true
-    | AppIdent _ _ (ident.Z_shiftr _) args => true
-    | _ => false
-    end.
-
-  Definition inline_shiftr_and_land {t} (e : Expr t) : Expr t :=
-    fun var => inline_op shift_land_matcher (e _).
-
-End InlineOperations.
-*)
+End PreFancy.
 
 Module MontgomeryReduction.
   Section MontRed'.
@@ -9206,8 +9305,8 @@ Module MontgomeryReduction.
     Context (nout : nat) (Hnout : nout = 2%nat).
 
     Definition montred' (lo_hi : (Z * Z)) :=
-      dlet_nd y := nth_default 0 (BaseConversion.widemul Zlog2R n nout (fst lo_hi) N') 0  in
-      dlet_nd t1_t2 := (BaseConversion.widemul Zlog2R n nout y N) in
+      dlet_nd y := nth_default 0 (BaseConversion.widemul_inlined Zlog2R n nout (fst lo_hi) N') 0  in
+      dlet_nd t1_t2 := (BaseConversion.widemul_inlined Zlog2R n nout y N) in
       dlet_nd sum_carry := Rows.add (weight Zlog2R 1) 2 [fst lo_hi; snd lo_hi] t1_t2 in
       dlet_nd y' := Z.zselect (snd sum_carry) 0 N in
       dlet_nd lo''_carry := Z.sub_get_borrow_full R (nth_default 0 (fst sum_carry) 1) y' in
@@ -9244,7 +9343,7 @@ Module MontgomeryReduction.
       rewrite Hlo, Hhi.
       assert (0 <= T mod R * N' < w 2) by (solve_range).
 
-      rewrite !BaseConversion.widemul_correct
+      rewrite !BaseConversion.widemul_inlined_correct
         by (rewrite ?BaseConversion.widemul_correct; autorewrite with push_nth_default; solve_range).
       rewrite Rows.add_partitions, Rows.add_div by (distr_length; apply wprops; omega).
       rewrite R_two_pow.
@@ -9297,7 +9396,6 @@ Module MontgomeryReduction.
     Context (N R N' : Z)
             (machine_wordsize : Z).
 
-    Let n : nat := Z.to_nat (Qceiling ((Z.log2_up N) / machine_wordsize)).
     Let bound := Some r[0 ~> (2^machine_wordsize - 1)%Z]%zrange.
 
     Definition relax_zrange_of_machine_wordsize
@@ -9308,11 +9406,7 @@ Module MontgomeryReduction.
 
     Definition check_args {T} (res : Pipeline.ErrorT T)
       : Pipeline.ErrorT T
-      := if (N =? 0)%Z
-         then Pipeline.Error (Pipeline.Values_not_provably_distinct "N ≠ 0" N 0)
-         else if (n =? 0)%Z
-              then Pipeline.Error (Pipeline.Values_not_provably_distinct "n ≠ 0" N 0)
-              else res.
+      := res. (* TODO: this should actually check stuff that corresponds with preconditions of montred'_correct *)
 
     Notation BoundsPipeline_correct in_bounds out_bounds op
       := (fun rv (rop : Expr (type.reify_type_of op)) Hrop
@@ -9355,51 +9449,113 @@ Module Montgomery256.
          As montred256_correct.
   Proof. Time solve_rmontred machine_wordsize. Time Qed.
 
-  Import Straightline.expr.
   Import PrintingNotations.
-  Set Printing Depth 1000000.
-  Local Notation "'tZ'" := (type.type_primitive type.Z).
-  Eval lazy in (Straightline.of_Expr montred256).
-  Print montred256.
+  Set Printing Width 10000.
 
-(* TODO: to get the right kind of output operation, I probably want
-  to inline all these shifts/ands. *)
-  (*
-montred256 = fun var : type -> Type => λ x : var (type.type_primitive type.Z * type.type_primitive type.Z)%ctype,
-             expr_let x0 := (uint128)(x₁ >> 128) in
-             expr_let x1 := ((uint128)(x₁) & 340282366920938463463374607431768211455) in
-             expr_let x2 := 79228162514264337593543950337 *₂₅₆ x0 in
-             expr_let x3 := ((uint128)(x2) & 340282366920938463463374607431768211455) in
-             expr_let x4 := 340282366841710300986003757985643364352 *₂₅₆ x1 in
-             expr_let x5 := ((uint128)(x4) & 340282366920938463463374607431768211455) in
-             expr_let x6 := (uint256)(x3 << 128) in
-             expr_let x7 := (uint256)(x5 << 128) in
-             expr_let x8 := 79228162514264337593543950337 *₂₅₆ x1 in
-             expr_let x9 := ADD_256 (x7, x8) in
-             expr_let x10 := ADD_256 (x6, x9₁) in
-             expr_let x11 := (uint128)(x10₁ >> 128) in
-             expr_let x12 := ((uint128)(x10₁) & 340282366920938463463374607431768211455) in
-             expr_let x13 := 79228162514264337593543950335 *₂₅₆ x11 in
-             expr_let x14 := (uint128)(x13 >> 128) in
-             expr_let x15 := ((uint128)(x13) & 340282366920938463463374607431768211455) in
-             expr_let x16 := 340282366841710300967557013911933812736 *₂₅₆ x12 in
-             expr_let x17 := (uint128)(x16 >> 128) in
-             expr_let x18 := ((uint128)(x16) & 340282366920938463463374607431768211455) in
-             expr_let x19 := 340282366841710300967557013911933812736 *₂₅₆ x11 in
-             expr_let x20 := (uint256)(x15 << 128) in
-             expr_let x21 := (uint256)(x18 << 128) in
-             expr_let x22 := 79228162514264337593543950335 *₂₅₆ x12 in
-             expr_let x23 := ADD_256 (x21, x22) in
-             expr_let x24 := ADDC_256 (x23₂, x14, x17) in
-             expr_let x25 := ADD_256 (x20, x23₁) in
-             expr_let x26 := ADDC_256 (x25₂, x19, x24₁) in
-             expr_let x27 := ADD_256 (x25₁, x₁) in
-             expr_let x28 := ADDC_256 (x27₂, x26₁, x₂) in
-             expr_let x29 := SELC (x28₂, 0, 115792089210356248762697446949407573530086143415290314195533631308867097853951) in
-             expr_let x30 := Z.cast uint256 @@ (fst @@ SUB_256 (x28₁, x29)) in
-             ADDM (x30, 0, 115792089210356248762697446949407573530086143415290314195533631308867097853951)
+  Print montred256.
+(*
+montred256 = fun var : type -> Type => (λ x : var (type.type_primitive type.Z * type.type_primitive type.Z)%ctype,
+    expr_let x0 := 79228162514264337593543950337 *₂₅₆ (uint128)(x₁ >> 128) in
+    expr_let x1 := 340282366841710300986003757985643364352 *₂₅₆ ((uint128)(x₁) & 340282366920938463463374607431768211455) in
+    expr_let x2 := (uint256)(((uint128)(x0) & 340282366920938463463374607431768211455) << 128) in
+    expr_let x3 := (uint256)(((uint128)(x1) & 340282366920938463463374607431768211455) << 128) in
+    expr_let x4 := 79228162514264337593543950337 *₂₅₆ ((uint128)(x₁) & 340282366920938463463374607431768211455) in
+    expr_let x5 := ADD_256 (x3, x4) in
+    expr_let x6 := ADD_256 (x2, x5₁) in
+    expr_let x7 := 79228162514264337593543950335 *₂₅₆ (uint128)(x6₁ >> 128) in
+    expr_let x8 := 340282366841710300967557013911933812736 *₂₅₆ ((uint128)(x6₁) & 340282366920938463463374607431768211455) in
+    expr_let x9 := 340282366841710300967557013911933812736 *₂₅₆ (uint128)(x6₁ >> 128) in
+    expr_let x10 := (uint256)(((uint128)(x7) & 340282366920938463463374607431768211455) << 128) in
+    expr_let x11 := (uint128)(x7 >> 128) in
+    expr_let x12 := (uint256)(((uint128)(x8) & 340282366920938463463374607431768211455) << 128) in
+    expr_let x13 := (uint128)(x8 >> 128) in
+    expr_let x14 := 79228162514264337593543950335 *₂₅₆ ((uint128)(x6₁) & 340282366920938463463374607431768211455) in
+    expr_let x15 := ADD_256 (x12, x14) in
+    expr_let x16 := ADDC_256 (x15₂, x11, x13) in
+    expr_let x17 := ADD_256 (x10, x15₁) in
+    expr_let x18 := ADDC_256 (x17₂, x9, x16₁) in
+    expr_let x19 := ADD_256 (x17₁, x₁) in
+    expr_let x20 := ADDC_256 (x19₂, x18₁, x₂) in
+    expr_let x21 := SELC (x20₂, 0, 115792089210356248762697446949407573530086143415290314195533631308867097853951) in
+    expr_let x22 := SUB_256 (x20₁, x21) in
+    ADDM (x22₁, 0, 115792089210356248762697446949407573530086143415290314195533631308867097853951))%expr
      : Expr (type.uncurry (type.type_primitive type.Z * type.type_primitive type.Z -> type.type_primitive type.Z))
-   *)
+*)
+
+  Import Straightline.expr.
+  Import PreFancy.
+
+  Definition montred256_straightline := Eval lazy in (fun var dummy_var x => Straightline.of_Expr montred256 var x dummy_var).
+
+  Definition constant_to_scalar var ident (x : Z) : option (@scalar var ident type.Z) :=
+    if x =? (BinInt.Z.shiftr N 128)
+    then Some (Cast uint128 (Shiftr 128 (Primitive (t:=type.Z) N)))
+    else if x =? (BinInt.Z.shiftr N' 128)
+         then Some (Cast uint128 (Shiftr 128 (Primitive (t:=type.Z) N')))
+         else if x =? (BinInt.Z.land N (2^128 - 1))
+              then Some (Cast uint128 (Land (2^128-1) (Primitive (t:=type.Z) N)))
+              else if x =? (BinInt.Z.land N' (2^128 - 1))
+                   then Some (Cast uint128 (Land (2^128-1) (Primitive (t:=type.Z) N')))
+                   else None.
+  
+  Definition montred256_prefancy :=
+    Eval vm_compute in (fun var dummy_var x =>
+                    @of_straightline var dummy_var machine_wordsize (constant_to_scalar var) _
+                                              (montred256_straightline var dummy_var x)).
+
+  Local Notation "'tZ'" := (type.type_primitive type.Z).
+  Local Notation "'RegMod'" := (Primitive (t:=type.Z) 115792089210356248762697446949407573530086143415290314195533631308867097853951).
+  Local Notation "'RegPInv'" := (Primitive (t:=type.Z) 115792089210356248768974548684794254293921932838497980611635986753331132366849).
+  Local Notation "'RegZero'" := (Primitive (t:=type.Z) 0).
+  Local Notation "$ x" := (Cast uint256 (Fst (Cast2 (uint256,bool) (Var (tZ * tZ) x)))) (at level 10, format "$ x").
+  Local Notation "$ x ₁" := (Cast uint256 (Fst (Var (tZ * tZ) x))) (at level 10, format "$ x ₁").
+  Local Notation "$ x ₂" := (Cast uint256 (Snd (Var (tZ * tZ) x))) (at level 10, format "$ x ₂").
+  Local Notation "carry{ $ x }" := (Cast bool (Snd (Cast2 (uint256, bool) (Var (tZ * tZ) x)))) (at level 10, format "carry{ $ x }").
+  Local Notation "Lower{ x }" := (Cast uint128 (Land 340282366920938463463374607431768211455 x)) (at level 10, format "Lower{ x }").
+  Local Notation "$ x" := (Cast uint256 (Var tZ x)) (at level 10, format "$ x").
+  Local Notation "$ x" := (Cast uint128 (Var tZ x)) (at level 10, format "$ x").
+  Local Notation "f @( y , x1 , x2 ); g "
+    := (LetInAppIdentZZ (uint256, bool) f (Pair x1 x2) (fun y => g)) (at level 10, g at level 200, format "f @( y ,  x1 ,  x2 ); '//' g ").
+  Local Notation "f @( y , x1 , x2 , x3 ); g "
+    := (LetInAppIdentZZ (uint256, bool) f (Pair (Pair x1 x2) x3) (fun y => g)) (at level 10, g at level 200, format "f @( y ,  x1 ,  x2 ,  x3 ); '//' g ").
+  Local Notation "f @( y , x1 , x2 ); g "
+    := (LetInAppIdentZ uint256 f (Pair x1 x2) (fun y => g)) (at level 10, g at level 200, format "f @( y ,  x1 ,  x2 ); '//' g ").
+  Local Notation "f @( y , x1 , x2 , x3 ); g "
+    := (LetInAppIdentZ uint256 f (Pair (Pair x1 x2) x3) (fun y => g)) (at level 10, g at level 200, format "f @( y ,  x1 ,  x2 ,  x3 ); '//' g ").
+  Local Notation "shiftL@( y , x , n ); g"
+    := (LetInAppIdentZ uint256 (shiftl n) (Lower{x}) (fun y => g)) (at level 10, g at level 200, format "shiftL@( y ,  x ,  n ); '//' g ").
+  Local Notation "shiftR@( y , x , n ); g"
+    := (LetInAppIdentZ uint128 (shiftr n) x (fun y => g)) (at level 10, g at level 200, format "shiftR@( y ,  x ,  n ); '//' g ").
+  Local Notation "'Ret' $ x" := (Scalar (Var tZ x)) (at level 10, format "'Ret'  $ x").
+  Local Notation "( x , y )" := (Pair x y) (at level 10, left associativity).
+  Print montred256_prefancy.
+  (*
+    mullh@(x0, RegPInv, $x₁);
+    mulhl@(x1, RegPInv, $x₁);
+    shiftL@(x2, $x0, 128);
+    shiftL@(x3, $x1, 128);
+    mulll@(x4, RegPInv, $x₁);
+    add@(x5, $x3, $x4);
+    add@(x6, $x2, $x5);
+    mullh@(x7, RegMod, $x6);
+    mulhl@(x8, RegMod, $x6);
+    mulhh@(x9, RegMod, $x6);
+    shiftL@(x10, $x7, 128);
+    shiftR@(x11, $x7, 128);
+    shiftL@(x12, $x8, 128);
+    shiftR@(x13, $x8, 128);
+    mulll@(x14, RegMod, $x6);
+    add@(x15, $x12, $x14);
+    addc@(x16, carry{$x15}, $x11, $x13);
+    add@(x17, $x10, $x15);
+    addc@(x18, carry{$x17}, $x9, $x16);
+    add@(x19, $x17, $x₁);
+    addc@(x20, carry{$x19}, $x18, $x₂);
+    sel@(x21, carry{$x20}, RegZero, RegMod);
+    sub@(x22, $x20, $x21);
+    addm@(x23, $x22, RegZero, RegMod);
+    Ret $x23
+  *)
 End Montgomery256.
 
 (* Extra-specialized ad-hoc pretty-printing *)
@@ -9424,30 +9580,30 @@ Module FancyPrintingNotations.
        (primitive 0)
        TT) (only printing, at level 9) : expr_scope.
   Notation "'$R'" := 115792089237316195423570985008687907853269984665640564039457584007913129639936 : expr_scope.
-  Notation "'Lower128{RegMod}'" :=
+  Notation "'c.Lower(RegMod)'" :=
     (AppIdent
        (primitive 79228162514264337593543950335)
        TT) (only printing, at level 9) : expr_scope.
-  Notation "'RegMod' '>>' '128'" :=
+  Notation "'c.Upper(RegMod)'" :=
     (AppIdent
        (primitive 340282366841710300967557013911933812736)
-       TT) (only printing, at level 9, format "'RegMod'  '>>'  '128'") : expr_scope.
-  Notation "'Lower128{RegMuLow}'" :=
+       TT) (only printing, at level 9) : expr_scope.
+  Notation "'c.Lower(RegMuLow)'" :=
     (AppIdent
        (primitive 340282366841710300930663525764514709507)
        TT) (only printing, at level 9) : expr_scope.
-  Notation "'RegMuLow' '>>' '128'" :=
+  Notation "'c.Upper(RegMuLow)'" :=
     (AppIdent
        (primitive 79228162514264337589248983038)
-       TT) (only printing, at level 9, format "'RegMuLow'  '>>'  '128'") : expr_scope.
-  Notation "'Lower128{RegPinv}'" :=
+       TT) (only printing, at level 9) : expr_scope.
+  Notation "'c.Lower(RegPinv)'" :=
     (AppIdent
        (primitive 79228162514264337593543950337)
        TT) (only printing, at level 9) : expr_scope.
-  Notation "'RegPinv' '>>' '128'" :=
+  Notation "'c.Upper(RegPinv)'" :=
     (AppIdent
        (primitive 340282366841710300986003757985643364352)
-       TT) (only printing, at level 9, format "'RegPinv'  '>>'  '128'") : expr_scope.
+       TT) (only printing, at level 9) : expr_scope.
   Notation "'uint256'"
     := (r[0 ~> 115792089237316195423570985008687907853269984665640564039457584007913129639935]%zrange) : ctype_scope.
   Notation "'uint128'"
@@ -9495,6 +9651,9 @@ Module FancyPrintingNotations.
   Notation "'c.Sub(' '$' n ',' x ',' y ');' f" :=
     (expr_let n := Z.cast uint256 @@ (fst @@ (Z.cast2 (uint256, _)%core @@ (Z.sub_get_borrow_concrete $R @@ (x, y)))) in
          f)%expr (at level 40, f at level 200, right associativity, format "'c.Sub(' '$' n ','  x ','  y ');' '//' f") : expr_scope.
+  Notation "'c.Sub(' '$' n ',' x ',' y ');' f" :=
+    (expr_let n := Z.cast2 (uint256, _)%core @@ (Z.sub_get_borrow_concrete $R @@ (x, y)) in
+         f)%expr (at level 40, f at level 200, right associativity, format "'c.Sub(' '$' n ','  x ','  y ');' '//' f") : expr_scope.
   Notation "'c.AddM(' '$ret' ',' x ',' y ',' z ');'" :=
     (Z.cast uint256 @@ (Z.add_modulo @@ (x, y, z)))%expr (at level 40, format "'c.AddM(' '$ret' ','  x ','  y ','  z ');'") : expr_scope.
   Notation "'c.ShiftR(' '$' n ',' x ',' y ');' f" :=
@@ -9503,15 +9662,17 @@ Module FancyPrintingNotations.
     (expr_let n := Z.cast _ @@ (Z.rshi_concrete $R m @@ (x, y)) in f)%expr (at level 40, f at level 200, right associativity, format "'[' 'c.Rshi(' '$' n ','  x ','  y ','  m ');' ']' '//' f") : expr_scope.
   Notation "'c.ShiftL(' '$' n ',' x ',' y ');' f" :=
     (expr_let n := Z.cast _ @@ (Z.shiftl y @@ x) in f)%expr (at level 40, f at level 200, right associativity, format "'[' 'c.ShiftL(' '$' n ','  x ','  y ');' ']' '//' f") : expr_scope.
+  Notation "'c.ShiftL(' '$' n ',' x ',' y ');' f" :=
+    (expr_let n := Z.cast _ @@ (Z.shiftl y @@ (Z.cast uint128 @@ (Z.land 340282366920938463463374607431768211455 @@ x))) in f)%expr (at level 40, f at level 200, right associativity, format "'[' 'c.ShiftL(' '$' n ','  x ','  y ');' ']' '//' f") : expr_scope.
   Notation "'c.Lower128(' '$' n ',' x ');' f" :=
     (expr_let n := Z.cast _ @@ (Z.land 340282366920938463463374607431768211455 @@ x) in f)%expr (at level 40, f at level 200, right associativity, format "'[' 'c.Lower128(' '$' n ','  x ');' ']' '//' f") : expr_scope.
-  Notation "'c.LowerHalf(' x ')'"
-    := (Z.cast uint128 @@ (Z.land 340282366920938463463374607431768211455))
-         (at level 10, only printing, format "c.LowerHalf( x )")
+  Notation "'c.Lower(' x ')'"
+    := (Z.cast uint128 @@ (Z.land 340282366920938463463374607431768211455 @@ x))
+         (at level 10, only printing, format "c.Lower( x )")
   : expr_scope.
-  Notation "'c.UpperHalf(' x ')'"
-    := (Z.cast uint128 @@ (Z.shiftr 340282366920938463463374607431768211455))
-         (at level 10, only printing, format "c.UpperHalf( x )")
+  Notation "'c.Upper(' x ')'"
+    := (Z.cast uint128 @@ (Z.shiftr 128 @@ x))
+         (at level 10, only printing, format "c.Upper( x )")
   : expr_scope.
   Notation "( v << count )"
     := (Z.cast _ @@ (Z.shiftl count @@ v)%expr)
@@ -9538,16 +9699,16 @@ c.Rshi($x1, RegZero, $x_hi, 255);
 c.Rshi($x2, $x_hi, $x_lo, 255);
 c.ShiftR($x3, $x2, 128);
 c.Lower128($x4, $x2);
-c.Mul128x128($x5, RegMuLow >> 128, $x4);
+c.Mul128x128($x5, c.Upper(RegMuLow), $x4);
 c.ShiftR($x6, $x5, 128);
 c.Lower128($x7, $x5);
-c.Mul128x128($x8, Lower128{RegMuLow}, $x3);
+c.Mul128x128($x8, c.Lower(RegMuLow), $x3);
 c.ShiftR($x9, $x8, 128);
 c.Lower128($x10, $x8);
-c.Mul128x128($x11, RegMuLow >> 128, $x3);
+c.Mul128x128($x11, c.Upper(RegMuLow), $x3);
 c.ShiftL($x12, $x7, 128);
 c.ShiftL($x13, $x10, 128);
-c.Mul128x128($x14, Lower128{RegMuLow}, $x4);
+c.Mul128x128($x14, c.Lower(RegMuLow), $x4);
 c.Add256($x15, $x13, $x14);
 c.Addc128($x16, $x15_hi, $x6, $x9);
 c.Add256($x17, $x12, $x15_lo);
@@ -9559,16 +9720,16 @@ c.Addc128($x22, $x21_hi, RegZero, $x20_lo);
 c.Rshi($x23, $x22_lo, $x21_lo, 1);
 c.ShiftR($x24, $x23, 128);
 c.Lower128($x25, $x23);
-c.Mul128x128($x26, Lower128{RegMod}, $x24);
+c.Mul128x128($x26, c.Lower(RegMod), $x24);
 c.ShiftR($x27, $x26, 128);
 c.Lower128($x28, $x26);
-c.Mul128x128($x29, RegMod >> 128, $x25);
+c.Mul128x128($x29, c.Upper(RegMod), $x25);
 c.ShiftR($x30, $x29, 128);
 c.Lower128($x31, $x29);
-c.Mul128x128($x32, RegMod >> 128, $x24);
+c.Mul128x128($x32, c.Upper(RegMod), $x24);
 c.ShiftL($x33, $x28, 128);
 c.ShiftL($x34, $x31, 128);
-c.Mul128x128($x35, Lower128{RegMod}, $x25);
+c.Mul128x128($x35, c.Lower(RegMod), $x25);
 c.Add256($x36, $x34, $x35);
 c.Addc256($x37, $x36_hi, $x27, $x30);
 c.Add256($x38, $x33, $x36_lo);
@@ -9584,36 +9745,28 @@ c.AddM($ret, $x43, RegZero, RegMod);
 
 Print Montgomery256.montred256.
 (*
-c.ShiftR($x0, $x_lo, 128);
-c.Lower128($x1, $x_lo);
-c.Mul128x128($x2, Lower128{RegPinv}, $x0);
-c.Lower128($x3, $x2);
-c.Mul128x128($x4, RegPinv >> 128, $x1);
-c.Lower128($x5, $x4);
-c.ShiftL($x6, $x3, 128);
-c.ShiftL($x7, $x5, 128);
-c.Mul128x128($x8, Lower128{RegPinv}, $x1);
-c.Add256($x9, $x7, $x8);
-c.Add256($x10, $x6, $x9_lo);
-c.ShiftR($x11, $x10_lo, 128);
-c.Lower128($x12, $x10_lo);
-c.Mul128x128($x13, Lower128{RegMod}, $x11);
-c.ShiftR($x14, $x13, 128);
-c.Lower128($x15, $x13);
-c.Mul128x128($x16, RegMod >> 128, $x12);
-c.ShiftR($x17, $x16, 128);
-c.Lower128($x18, $x16);
-c.Mul128x128($x19, RegMod >> 128, $x11);
-c.ShiftL($x20, $x15, 128);
-c.ShiftL($x21, $x18, 128);
-c.Mul128x128($x22, Lower128{RegMod}, $x12);
-c.Add256($x23, $x21, $x22);
-c.Addc256($x24, $x23_hi, $x14, $x17);
-c.Add256($x25, $x20, $x23_lo);
-c.Addc256($x26, $x25_hi, $x19, $x24_lo);
-c.Add256($x27, $x25_lo, $x_lo);
-c.Addc256($x28, $x27_hi, $x26_lo, $x_hi);
-c.Selc($x29, $x28_hi, RegZero, RegMod);
-c.Sub($x30, $x28_lo, $x29);
-c.AddM($ret, $x30, RegZero, RegMod);
+c.Mul128x128($x0, c.Lower(RegPinv), c.Upper($x_lo));
+c.Mul128x128($x1, c.Upper(RegPinv), c.Lower($x_lo));
+c.ShiftL($x2, $x0, 128);
+c.ShiftL($x3, $x1, 128);
+c.Mul128x128($x4, c.Lower(RegPinv), c.Lower($x_lo));
+c.Add256($x5, $x3, $x4);
+c.Add256($x6, $x2, $x5_lo);
+c.Mul128x128($x7, c.Lower(RegMod), c.Upper($x6_lo));
+c.Mul128x128($x8, c.Upper(RegMod), c.Lower($x6_lo));
+c.Mul128x128($x9, c.Upper(RegMod), c.Upper($x6_lo));
+c.ShiftL($x10, $x7, 128);
+c.ShiftR($x11, $x7, 128);
+c.ShiftL($x12, $x8, 128);
+c.ShiftR($x13, $x8, 128);
+c.Mul128x128($x14, c.Lower(RegMod), c.Lower($x6_lo));
+c.Add256($x15, $x12, $x14);
+c.Addc256($x16, $x15_hi, $x11, $x13);
+c.Add256($x17, $x10, $x15_lo);
+c.Addc256($x18, $x17_hi, $x9, $x16_lo);
+c.Add256($x19, $x17_lo, $x_lo);
+c.Addc256($x20, $x19_hi, $x18_lo, $x_hi);
+c.Selc($x21, $x20_hi, RegZero, RegMod);
+c.Sub($x22, $x20_lo, $x21);
+c.AddM($ret, $x22_lo, RegZero, RegMod);
  *)
